elo-coq/ProgressPreservation.v
@@ -4,9 +4,9 @@ From Elo Require Export Core.
 
 (* Auxiliary Lemmas *)
 
-Definition well_typed_memory D (mt : list typ) (m : mem) :=
+Definition well_typed_memory (mt : list typ) (m : mem) :=
   length mt = length m /\
-  (forall i, D / mt / empty |-- (get_tm m i) is (get_typ mt i)).
+  (forall i, mt / empty |-- (get_tm m i) is (get_typ mt i)).
 
 Inductive extends' : list typ -> list typ -> Prop :=
   | extends_nil : forall mt,
@@ -59,10 +59,10 @@ Proof.
   induction mt; auto using extends'.
 Qed.
 
-Lemma memory_weakening : forall D mt mt' Gamma t T, 
+Lemma memory_weakening : forall mt mt' Gamma t T, 
   mt extends mt' ->
-  D / mt' / Gamma |-- t is T ->  
-  D / mt  / Gamma |-- t is T.
+  mt' / Gamma |-- t is T ->  
+  mt  / Gamma |-- t is T.
 Proof.
   intros * Hext Htype.
   induction Htype; eauto using @typeof.
@@ -70,31 +70,31 @@ Proof.
   erewrite extends_lookup; auto using T_Loc.
 Qed.
 
-Lemma context_weakening : forall D mt Gamma Gamma' t T,
+Lemma context_weakening : forall mt Gamma Gamma' t T,
   Gamma includes Gamma' ->
-  D / mt / Gamma' |-- t is T ->
-  D / mt / Gamma  |-- t is T.
+  mt / Gamma' |-- t is T ->
+  mt / Gamma  |-- t is T.
 Proof.
   intros * Hinc Htype.
   generalize dependent Gamma.
   induction Htype; intros * Hinc;
-  eauto using @typeof, update_preserves_inclusion.
+  eauto 6 using @typeof, update_preserves_inclusion.
 Qed.
 
-Lemma context_weakening_empty : forall D mt Gamma t T,
-  D / mt / empty |-- t is T ->
-  D / mt / Gamma |-- t is T.
+Lemma context_weakening_empty : forall mt Gamma t T,
+  mt / empty |-- t is T ->
+  mt / Gamma |-- t is T.
 Proof.
   intros * Htype.
-  eapply (context_weakening _ _ _ empty); auto.
+  eapply (context_weakening _ _ empty); auto.
   discriminate.
 Qed.
 
-Lemma assignment_preserves_memory_typing : forall D m mt t i,
+Lemma assignment_preserves_memory_typing : forall m mt t i,
   i < length m ->
-  well_typed_memory D mt m ->
-  D / mt / empty |-- t is (get_typ mt i) ->
-  well_typed_memory D mt (set m i t).
+  well_typed_memory mt m ->
+  mt / empty |-- t is (get_typ mt i) ->
+  well_typed_memory mt (set m i t).
 Proof.
   intros * Hi [Hlen Htype1] Htype2. split.
   - rewrite Hlen. apply set_preserves_length.
@@ -105,10 +105,10 @@ Proof.
       erewrite (get_set_i_neq_j TM_Nil); auto.
 Qed.
 
-Lemma substitution_preserves_typing : forall D mt Gamma id t u T U,
-  D / mt / (update Gamma id U) |-- t is T ->
-  D / mt / empty |-- u is U ->
-  D / mt / Gamma |-- [id := u] t is T.
+Lemma substitution_preserves_typing : forall mt Gamma id t u T U,
+  mt / (update Gamma id U) |-- t is T ->
+  mt / empty |-- u is U ->
+  mt / Gamma |-- [id := u] t is T.
 Proof.
   intros * Ht Hu.
   generalize dependent T.
@@ -136,16 +136,23 @@ Proof.
       rewrite <- H1.
       symmetry. apply lookup_update_idempotent.
       assumption.
-  - apply T_LetVal.
-    + auto.
-    + destruct String.eqb eqn:E in *.
+  - destruct String.eqb eqn:E in *; apply T_LetVal; eauto.
+    + apply String.eqb_eq in E. subst.
+      eauto using context_weakening, update_overwrite.
+    + apply String.eqb_neq in E.
+      eauto using context_weakening, update_permutation.
+  - destruct String.eqb eqn:E in *; apply T_LetVar; eauto.
+    + apply String.eqb_eq in E. subst.
+      eauto using context_weakening, update_overwrite.
+    + apply String.eqb_neq in E.
+      eauto using context_weakening, update_permutation.
+  - apply T_LetFun.
+    + destruct String.eqb eqn:E.
       * apply String.eqb_eq in E. subst.
         eauto using context_weakening, update_overwrite.
       * apply String.eqb_neq in E.
         eauto using context_weakening, update_permutation.
-  - apply T_LetVar.
-    + auto.
-    + destruct String.eqb eqn:E in *.
+    + destruct String.eqb eqn:E.
       * apply String.eqb_eq in E. subst.
         eauto using context_weakening, update_overwrite.
       * apply String.eqb_neq in E.
@@ -158,14 +165,14 @@ Lemma length_add : forall {A B} (l1 : list A) (l2 : list B) a b,
 Proof.
 Admitted.
 
-Theorem preservation : forall D D' m m' mt t t' T,
-  D / mt / empty |-- t is T ->
-  well_typed_memory D mt m ->
-  D / m / t --> D' / m' / t' ->
+Theorem preservation : forall m m' mt t t' T,
+  mt / empty |-- t is T ->
+  well_typed_memory mt m ->
+  m / t --> m' / t' ->
   exists mt',
     mt' extends mt /\
-    D' / mt' / empty |-- t' is T /\
-    well_typed_memory D' mt' m'.
+    mt' / empty |-- t' is T /\
+    well_typed_memory mt' m'.
 Proof.
   remember empty as Gamma.
   intros * Htype.
@@ -173,61 +180,47 @@ Proof.
   induction Htype; intros ?t' Hmem Hstep;
   inversion Hstep; subst.
   (* T_Asg *)
-  * eapply IHHtype2 in H6; auto.
-    destruct H6 as [mt' [Hext [Htype' Hmem']]].
+  * eapply IHHtype2 in H4; trivial.
+    destruct H4 as [mt' [Hext [Htype' Hmem']]].
     exists mt'. split; try split; eauto using memory_weakening, T_Asg.
-  * eapply IHHtype1 in H7; auto.
-    destruct H7 as [mt' [Hext [Htype' Hmem']]].
+  * eapply IHHtype1 in H5; trivial.
+    destruct H5 as [mt' [Hext [Htype' Hmem']]].
     exists mt'. split; try split; eauto using memory_weakening, T_Asg.
   * exists mt. split. apply extends_refl. split. apply T_Nil.
     eapply assignment_preserves_memory_typing; auto.
     inversion Htype1. subst. eauto.
   (* T_Call *)
-  * eapply IHHtype in H7; trivial.
-    destruct H7 as [mt' [Hextends [Htype' Hmem']]].
+  * eapply IHHtype2 in H4; trivial.
+    destruct H4 as [mt' [Hextends [Htype' Hmem']]].
     exists mt'. split; trivial.
     split; try eapply T_Call; eauto using memory_weakening.
-  * exists mt. split; only 1 : apply extends_refl.
-    split; trivial. rewrite H in H8. injection H8 as ?; subst.
-    eapply substitution_preserves_typing.
-    ** admit.
-    ** apply Htype.
+  * exists mt. inversion Htype1. subst.
+    split; only 1 : apply extends_refl.
+    split; only 2 : trivial.
+    eapply substitution_preserves_typing; eauto.
+    admit.
   (* T_Seq *)
-  * specialize (IHHtype1 eq_refl t2 Hmem H6).
+  * specialize (IHHtype1 eq_refl t2 Hmem H4).
     destruct IHHtype1 as [mt' [? [? ?]]].
     exists mt'. split. assumption.
     split; eauto using T_Seq, memory_weakening.
   * exists mt. split. apply extends_refl. split; assumption.
   (* T_LetVal *)
-  * specialize (IHHtype1 eq_refl e' Hmem H8).
+  * specialize (IHHtype1 eq_refl e' Hmem H6).
     destruct IHHtype1 as [mt' [Hextends [Htype' Hmem']]].
     exists mt'. split. assumption.
     split; eauto using T_LetVal, memory_weakening.
-  * exists mt. split.
-    ** apply extends_refl.
-    ** split. eapply substitution_preserves_typing.
-       *** apply Htype2.
-       *** destruct Hmem as [Hlen Hmem2].
-           specialize (Hmem2 i).
-           admit.
-       *** destruct Hmem as [Hlen H]. split.
-           admit. admit.
+  * exists mt. split. apply extends_refl. split; auto.
+    eapply substitution_preserves_typing; eauto.
   (* T_LetVar *)
-  * specialize (IHHtype1 eq_refl e' Hmem H8).
+  * specialize (IHHtype1 eq_refl e' Hmem H6).
     destruct IHHtype1 as [mt' [Hextends [Htype' Hmem']]].
     exists mt'. split. assumption.
     split; eauto using T_LetVar, memory_weakening.
-  * exists (add mt A). split.
-    ** apply extends_add.
-    ** split.
-      *** eapply substitution_preserves_typing.
-         assert (add mt A extends mt). { apply extends_add. }
-         eapply (memory_weakening _ _ _ _ _ _ H Htype2).
-         admit.
-      *** destruct Hmem as [Hlen H]. split.
-         **** apply length_add. auto.
-         **** intros j. specialize (H j).
-             admit.
+  * exists (add mt E). split. apply extends_add. split.
+    ** admit.
+    ** destruct Hmem as [Hlen Htype]. admit. (* easy *)
+  * admit.
   * admit.
   * admit.
   * admit.
